Swap Term and Typ to match the usual convention

Main.lean
@@ -29,32 +29,30 @@ deriving BEq
 Terms in our toy language
 
 We hardcode all the inductive type constructors and eliminators here instead of implementing them separately as axioms (which would significantly simplify the type checker) to prevent adversies from writing fake proofs that use arbitrary axioms
-
-The other advantage of that approach is that it enables us to write an evaluator for this toy language, which admittedly isn't very useful
 -/
 inductive Term
   /-- Variable -/
   | var : String → Term
   /-- Lambda -/
-  | lam : String → Typ × Term → Term
+  | lam : String → Term × Typ → Term
   /-- Function application -/
-  | app : Typ × Term → Typ × Term → Term
+  | app : Term × Typ → Term × Typ → Term
   /-- Construct a product -/
-  | and : Typ × Term → Typ × Term → Term
+  | and : Term × Typ → Term × Typ → Term
   /-- Get first element of product -/
-  | and1 : Typ × Term → Term
+  | and1 : Term × Typ → Term
   /-- Get second element of product -/
-  | and2 : Typ × Term → Term
+  | and2 : Term × Typ → Term
   /-- Construct a sum -/
-  | or : Typ × Term → Term
+  | or : Term × Typ → Term
   /-- Zero as a nat -/
   | zero : Term
   /-- One or greater as a nat -/
-  | succ : Typ × Term → Term
+  | succ : Term × Typ → Term
   /-- Eliminator (recursor) for nats -/
-  | nat_elim : Typ → Typ × Term → Typ × Term → Typ × Term → Term
+  | nat_elim : Typ → Term × Typ → Term × Typ → Term × Typ → Term
   /-- Eliminator for false -/
-  | fls_elim : Typ × Term → Term
+  | fls_elim : Term × Typ → Term
 
 def Typ.toString : Typ → String
   | new α => s!"(list 0n \"{α}\")"
@@ -67,112 +65,119 @@ def Typ.toString : Typ → String
 instance : ToString Typ := ⟨Typ.toString⟩
 
 mutual
-def toString (t : Typ × Term) := s!"(cons {t.1} {t.2.toString})"
+def toString (t : Term × Typ) := s!"(cons {t.1.toString} {t.2})"
 
 def Term.toString : Term → String
   | .var x => s!"(list 10n '{x})"
   | .lam x b => s!"(list 11n '{x} {toString b})"
-  | .app f x => s!"(list 12n {toString f} {toString x})"
+  | .app f a => s!"(list 12n {toString f} {toString a})"
   | .and x y => s!"(list 13n {toString x} {toString y})"
   | .and1 x => s!"(list 14n {toString x})"
-  | .and2 y => s!"(list 15n {toString y})"
+  | .and2 x => s!"(list 15n {toString x})"
   | .or z => s!"(list 16n {toString z})"
   | .zero => s!"'(17n)"
-  | .succ x => s!"(list 18n {toString x})"
-  | .nat_elim τ a b c => s!"(list 19n {τ} {toString a} {toString b} {toString c})"
+  | .succ n => s!"(list 18n {toString n})"
+  | .nat_elim α n x f => s!"(list 19n {α} {toString n} {toString x} {toString f})"
   | .fls_elim x => s!"(list 20n {toString x})"
 end
 
-instance : ToString (Typ × Term) := ⟨toString⟩
+instance : ToString (Term × Typ) := ⟨toString⟩
 
 instance : ToString Term := ⟨Term.toString⟩
 
 /--
 The type checker!
 
-TODO: Port to Lurk
+The variable names are chosen intentionally so that i.e. `a : Term` corresponds to `α : Typ`.
 -/
-def check (env : Std.HashMap String Typ) : Typ → Term → Bool
-  | τ, .var x =>
-    (· == τ) <$> env[x]? |>.getD false
-  | .fn α β, .lam x (β', b) =>
-    β' == β && check (env.insert x α) β' b
-  | τ, .app (.fn α β, f) (α', x) =>
-    α' == α && β == τ && check env (.fn α β) f && check env α' x
-  | .prod α β, .and (α', x) (β', y) =>
-    α' == α && β' == β && check env α' x && check env β' y
-  | τ, .and1 (.prod α β, x) =>
-    τ == α && check env (.prod α β) x
-  | τ, .and2 (.prod α β, y) =>
-    τ == β && check env (.prod α β) y
-  | .sum α β, .or (γ, z) =>
-    (γ == α || γ == β) && check env γ z
-  | .nat, .zero =>
+def check (env : Std.HashMap String Typ) : Term → Typ → Bool
+  | .var x, α =>
+    (· == α) <$> env[x]? |>.getD false
+  | .lam x (b, β), .fn α β' =>
+    β' == β && check (env.insert x α) b β
+  | .app (f, .fn α β) (a, α'), β' =>
+    α' == α && β' == β && check env f (.fn α β) && check env a α
+  | .and (a, α) (b, β), .prod α' β' =>
+    α' == α && β' == β && check env a α && check env b β
+  | .and1 (x, .prod α β), α' =>
+    α' == α && check env x (.prod α β)
+  | .and2 (x, .prod α β), β' =>
+    β' == β && check env x (.prod α β)
+  | .or (c, γ), .sum α β =>
+    (γ == α || γ == β) && check env c γ
+  | .zero, .nat =>
     true
-  | .nat, .succ (α, x) =>
-    α == .nat && check env α x
-  | .fn .nat τ, .nat_elim α (.nat, a) (β, b) (.fn .nat (.fn γ δ), c) =>
-    τ == α && τ == β && τ == γ && τ == δ && check env .nat a && check env β b && check env (.fn .nat (.fn γ δ)) c
-  | _, .fls_elim (.fls, _) =>
+  | .succ (n, .nat), .nat =>
+    check env n .nat
+  | .nat_elim α (n, .nat) (b, β) (f, .fn .nat (.fn γ δ)), .fn .nat τ =>
+    τ == α && τ == β && τ == γ && τ == δ && check env n .nat && check env b β && check env f (.fn .nat (.fn γ δ))
+  | .fls_elim (_, .fls), _ =>
     true
   | _, _ =>
     false
 
-theorem false_empty : check (.ofList []) .fls t == false := by
+theorem false_empty : check (.ofList []) t .fls == false := by
   sorry
 
 -- TODO: Implement eval so we can state 2 + 2 = 4
--- def eval env (venv : Std.HashMap String Term) τ t (h : check env τ t) (henv : ∀ x, x ∈ env.keys → x ∈ venv.keys) : Term :=
---   match τ, t with
---   | _, .var x =>
---     venv[x]'(by sorry)
---   | .fn α β, .lam x (β', b) =>
---     .lam x (eval (env.insert x α) venv β b (by sorry) (by sorry))
---   | .app (.fn α β, f) (α', x) =>
---     eval
+-- def eval env (venv : Std.HashMap String Term) t τ (h : check env t τ) (henv : ∀ x, x ∈ venv.keys → x ∈ env.keys) : Term × Typ :=
+--   match t, τ with
+--   | .var x, _ =>
+--     (venv[x]'(by sorry), env[x]'(by sorry))
+--   | .lam f (b, β'), .fn α β =>
+--     (.lam f (eval (env.insert f α) venv b β (by sorry) (by sorry)), .fn α β)
+--   | .app (f, .fn α β) (a, α'), β' =>
+--     let (a', α'') := eval env venv a α h henv
+--     let (f', _) := eval env venv f (.fn α β) h henv
+--     match f' with
+--     | .lam x (b, β'') => eval (env.insert x α) (venv.insert x a') b β (by sorry) (by sorry)
+--     | _ => nofun
+--   | .and (a, α) (b, β), τ =>
+--     (.and (eval env venv a α (by sorry) henv) (eval env venv b β (by sorry) henv), τ)
 
-def a_imp_a := (Typ.fn (.new "A") (.new "A"), Term.lam "a" (.new "A", .var "a"))
+
+def a_imp_a := (Term.lam "a" (.var "a", .new "A"), Typ.fn (.new "A") (.new "A"))
 
 #guard check (.ofList []) a_imp_a.1 a_imp_a.2
 
 #eval IO.println a_imp_a
 
 /-- A → B → B ∧ A -/
-def a_imp_b_imp_ba := (Typ.fn (.new "A") (.fn (.new "B") (.prod (.new "B") (.new "A"))), Term.lam "a" (.fn (.new "B") (.prod (.new "B") (.new "A")), .lam "b" (.prod (.new "B") (.new "A"), .and (.new "B", .var "b") (.new "A", .var "a"))))
+def a_imp_b_imp_ba := (Term.lam "a" (.lam "b" (.and (.var "b", .new "B") (.var "a", .new "A"), .prod (.new "B") (.new "A")), .fn (.new "B") (.prod (.new "B") (.new "A"))), Typ.fn (.new "A") (.fn (.new "B") (.prod (.new "B") (.new "A"))))
 
 #guard check (.ofList []) a_imp_b_imp_ba.1 a_imp_b_imp_ba.2
 
 #eval IO.println a_imp_b_imp_ba
 
 /-- A ∧ B → B ∧ A -/
-def ab_imp_ba := (Typ.fn (.prod (.new "A") (.new "B")) (.prod (.new "B") (.new "A")), Term.lam "ab" (.prod (.new "B") (.new "A"), .and (.new "B", .and2 (.prod (.new "A") (.new "B"), .var "ab")) (.new "A", .and1 (.prod (.new "A") (.new "B"), .var "ab"))))
+def ab_imp_ba := (Term.lam "ab" (.and (.and2 (.var "ab", .prod (.new "A") (.new "B")), .new "B") (.and1 (.var "ab", .prod (.new "A") (.new "B")), .new "A"), .prod (.new "B") (.new "A")), Typ.fn (.prod (.new "A") (.new "B")) (.prod (.new "B") (.new "A")))
 
 #guard check (.ofList []) ab_imp_ba.1 ab_imp_ba.2
 
 #eval IO.println ab_imp_ba
 
 /-- ¬(A ∨ B) → ¬A -/
-def not_ab_imp_not_a := (Typ.fn (.fn (.sum (.new "A") (.new "B")) .fls) (.fn (.new "A") .fls), Term.lam "f" (.fn (.new "A") .fls, .lam "x" (.fls, .app (.fn (.sum (.new "A") (.new "B")) .fls, .var "f") (.sum (.new "A") (.new "B"), .or (.new "A", .var "x")))))
+def not_ab_imp_not_a := (Term.lam "f" (.lam "a" (.app (.var "f", .fn (.sum (.new "A") (.new "B")) .fls) (.or (.var "a", .new "A"), .sum (.new "A") (.new "B")), .fls), .fn (.new "A") .fls), Typ.fn (.fn (.sum (.new "A") (.new "B")) .fls) (.fn (.new "A") .fls))
 
 #guard check (.ofList []) not_ab_imp_not_a.1 not_ab_imp_not_a.2
 
 #eval IO.println not_ab_imp_not_a
 
 /-- 2 exists (yeah I know this is not super exciting) -/
-def two := (Typ.nat, Term.succ (.nat, (.succ (.nat, .zero))))
+def two := (Term.succ ((.succ (.zero, .nat)), .nat), Typ.nat)
 
 #guard check (.ofList []) two.1 two.2
 
 /-- 4 exists -/
-def four := (Typ.nat, Term.succ (.nat, (.succ two)))
+def four := (Term.succ (.succ two, .nat), Typ.nat)
 
 #guard check (.ofList []) four.1 four.2
 
 /-- Addition -/
-def add := (Typ.fn .nat (.fn .nat .nat), Term.lam "a" (.fn .nat .nat, .nat_elim .nat (.nat, .zero) (.nat, .var "a") (.fn .nat (.fn .nat .nat), .lam "_" (.fn .nat .nat, .lam "b" (.nat, .succ (.nat, .var "b"))))))
+def add := (Term.lam "a" (.nat_elim .nat (.zero, .nat) (.var "a", .nat) (.lam "_" (.lam "b" (.succ (.var "b", .nat), .nat), .fn .nat .nat), .fn .nat (.fn .nat .nat)), .fn .nat .nat), Typ.fn .nat (.fn .nat .nat))
 
 #guard check (.ofList []) add.1 add.2
 
-def two_plus_two := (Typ.nat, Term.app (.fn .nat .nat, .app add two) two)
+def two_plus_two := (Term.app (.app add two, .fn .nat .nat) two, Typ.nat)
 
 #guard check (.ofList []) two_plus_two.1 two_plus_two.2
